implement constraints as finsets, allowing subset proofs to get implications about subsets of constraints (e.g. addOperation to addChip)

SP1Foundations/Constraint.lean
@@ -1,13 +1,39 @@
 import SP1Foundations.Field
 import SP1Foundations.ByteOpcode
 
+inductive AirInteraction.Kind where
+  | BYTE
+  | MEMORY
+  | PROGRAM
+  | STATE
+
+-- structure AirInteraction where
+--   mult : ℕ
+
+structure ByteAirInteraction where
+  mk_air ::
+  op : ByteOpcode
+  x : BabyBear
+  y : BabyBear
+  z : BabyBear
+  mult : BabyBear
+
+def ByteAirInteraction.to_result : ByteAirInteraction → Unit
+  | .mk_air (op := .AND) x y z mult => ()
+  | .mk_air .OR x y z mult => ()
+  | .mk_air .XOR x y z mult => ()
+  | _ => ()
+
 inductive SP1Constraint where
-  /-- Assertion that a particular value is real. -/
+  /-- Assertion that a particular value is zero. -/
   | assertZero (x : BabyBear)
   /-- Sending air interactions with `kind == byte` -/
-  | sendAirInteraction_byte (op : ByteOpcode)
-      (x y z : BabyBear) (mult : ℕ)
+  | sendAirInteraction_byte (op : ByteOpcode) (x y z : BabyBear) (mult : ℕ)
   -- TODO: other air interactions
+
+instance : DecidableEq SP1Constraint
+  | (SP1Constraint.assertZero x), (SP1Constraint.assertZero y) => sorry
+  | _, _ => sorry
 
 namespace SP1Constraint
 
@@ -27,13 +53,32 @@ def toProp : SP1Constraint → Prop
 
 end SP1Constraint
 
-@[reducible] def constraintList_toProp (cs : List SP1Constraint) : Prop :=
+section constraintSet
+
+-- TODO: should this exist? maybe even as `abbrev`?
+@[reducible] def constraintSet := Finset SP1Constraint
+
+/-- Covert a set of constraints to a single proposition stating that they all hold. -/
+def constraintSet_toProp (cs : Finset SP1Constraint) : Prop :=
   ∀ constraint ∈ cs, constraint.toProp
 
-@[simp] lemma constraintList_toProp_nil :
-    constraintList_toProp [] = True := by
-  simp [constraintList_toProp]
+@[simp] lemma constraintSet_toProp_empty : constraintSet_toProp ∅ = True := by
+  simp [constraintSet_toProp]
 
-@[simp] lemma constraintList_toProp_cons (c : SP1Constraint) (cs : List SP1Constraint) :
-    constraintList_toProp (c :: cs) = (c.toProp ∧ constraintList_toProp cs) := by
-  simp [constraintList_toProp]
+@[simp] lemma constraintSet_toProp_singleton (c : SP1Constraint) : constraintSet_toProp {c} = c.toProp := by
+  simp [constraintSet_toProp]
+
+@[simp] lemma constraintSet_toProp_insert (c : SP1Constraint) (cs : Finset SP1Constraint) :
+    constraintSet_toProp (insert c cs) = (c.toProp ∧ constraintSet_toProp cs) := by
+  simp [constraintSet_toProp]
+
+lemma toProp_of_mem_constraintSet (cs : Finset SP1Constraint) (c : SP1Constraint) :
+    c ∈ cs → constraintSet_toProp cs → c.toProp := by
+  sorry
+
+/-- A larger set of constraints `cs'` implies a smaller set of constraints `cs`. -/
+lemma toProp_imp_of_constraintSet_subset' (cs cs' : Finset SP1Constraint)
+    (h : cs ⊆ cs') : constraintSet_toProp cs' → constraintSet_toProp cs := by
+  refine fun csp c h' => csp c (h h')
+
+end constraintSet
